TM/Code/BoolTM.v
@@ -1,6 +1,5 @@
-Require Import Prelim TM.TM TM.Code.Code TM.Code.CodeTM.
-Require Import Program.Equality.
-
+Require Import TM.Prelim TM.TM TM.Code.Code TM.Code.CodeTM.
+Require Import TM.Combinators.SequentialComposition TM.Basic.Mono TM.Basic.Basic.
 
 Open Scope vector_scope.
 
@@ -9,7 +8,7 @@ Section Neg_TM.
 
   Variable (F : finType) (def : bool_fin -> F).
 
-  Definition neg_TM_trans :
+  Definition bool_neg_TM_trans :
     bool_fin * (Vector.t (option bool_fin) 1) ->
     bool_fin * (Vector.t (option bool_fin * move) 1).
   Proof.
@@ -21,26 +20,26 @@ Section Neg_TM.
       + (* None       *) constructor. apply true. constructor. apply (None,       N). constructor.
   Defined.
 
-  Definition neg_TM : mTM bool_fin 0.
+  Definition bool_neg_TM : mTM bool_fin 0.
   Proof.
     split with (states := bool_fin).
-    - apply neg_TM_trans.
+    - apply bool_neg_TM_trans.
     - apply false.
     - apply id.
   Defined.
 
-  Definition neg_mTM : { M : mTM bool_fin 0 & states M -> F} := (neg_TM; def).
+  Definition bool_neg_mTM : { M : mTM bool_fin 0 & states M -> F} := (bool_neg_TM; def).
 
-  Lemma neg_TM_onestep (inittapes : tapes bool_fin 1) :
-    cstate (step (M := neg_TM) (initc neg_TM inittapes)) = true.
+  Lemma bool_neg_TM_onestep (inittapes : tapes bool_fin 1) :
+    cstate (step (M := bool_neg_TM) (initc bool_neg_TM inittapes)) = true.
   Proof.
-    unfold initc, step, neg_TM in *. cbn in *.
-    dependent induction inittapes. dependent induction inittapes. cbn in *. clear IHinittapes.
+    destruct_tapes.
+    unfold initc, step, bool_neg_TM in *. cbn in *.
     destruct (current h); cbn; auto. destruct e; cbn; auto.
   Qed.
 
-  Lemma neg_TM_computes_sem :
-    neg_mTM ⊫ computes_locally_R_p (F := F) Fin.F1 Fin.F1 _ _ negb.
+  Lemma bool_neg_TM_computes_sem :
+    bool_neg_mTM ⊫ computes_locally_R_p (F := F) Fin.F1 Fin.F1 _ _ negb.
   Proof.
     hnf. intros inittapes i (b, outt) HLoop. cbn in *.
     assert (i >= 1).
@@ -50,31 +49,31 @@ Section Neg_TM.
     pose proof loop_fulfills_p HLoop as H_Stop. cbn in *. destruct b; auto.
     unfold loopM in *.
     erewrite (loop_ge (k1 := 1) (k2 := i)) in HLoop. Focus 2. omega. Focus 2.
-    cbn. unfold id. unfold neg_TM. cbn. rewrite neg_TM_onestep. reflexivity. inv HLoop.
-    apply computes_locally_R_iff. hnf. intros x (rest1&E1).
-    unfold initc, step, neg_TM in *. cbn in *.
-    dependent induction inittapes. dependent induction inittapes. cbn in *. clear IHinittapes.
-    hnf.
+    cbn. unfold id. unfold bool_neg_TM. cbn. rewrite bool_neg_TM_onestep. reflexivity. inv HLoop.
+    hnf. intros x (rest1&E1).
+    unfold initc, step, bool_neg_TM in *. cbn in *.
+    destruct_tapes.
+    hnf in *. unfold tape_encodes_locally_rest in *.
     destruct x; cbn in *;
       erewrite !tape_local_current_cons in H1; eauto; cbn in *; inv H1; cbn in *; now eauto.
   Qed.
 
-  Lemma neg_TM_computes_terminates_in :
-    neg_TM ↓ (fun _ => fun t => t = 1).
+  Lemma bool_neg_TM_computes_terminates_in :
+    bool_neg_TM ↓ (fun _ => fun t => t = 1).
   Proof.
-    hnf. intros inittape i ->. cbn. unfold id. rewrite neg_TM_onestep. eauto.
+    hnf. intros inittape i ->. cbn. unfold id. rewrite bool_neg_TM_onestep. eauto.
   Qed.
 
-  Lemma neq_TM_computes_total :
-    neg_mTM ⊨(1) computes_locally_R_p (F := F) Fin.F1 Fin.F1 _ _ negb.
+  Lemma bool_neq_TM_computes_total :
+    bool_neg_mTM ⊨(1) computes_locally_R_p (F := F) Fin.F1 Fin.F1 _ _ negb.
   Proof.
     hnf. intros inittape.
-    dependent induction inittape. dependent induction inittape. clear IHinittape; cbn in *.
-    unfold id. rewrite neg_TM_onestep. econstructor. split. eauto.
+    destruct_tapes. cbn in *.
+    rewrite bool_neg_TM_onestep. econstructor. split. cbn. eauto.
     hnf. intros x.
-    rewrite !tape_encodes_locally_iff. unfold tape_encodes_locally'. intros (tape&bl). cbn in *.
+    unfold tape_encodes_locally, tape_encodes_locally_rest in *. intros (tape&bl). cbn in *.
     destruct x; cbn in *; exists tape;
-      cbn; unfold neg_TM, step; cbn;
+      cbn; unfold bool_neg_TM, step; cbn;
         erewrite tape_local_current_cons; eauto; cbn; f_equal; eapply tape_local_right; eauto.
   Qed.
   
@@ -86,7 +85,7 @@ Section Copy.
 
   Variable (F : finType) (def : bool_fin -> F).
 
-  Definition copy_TM_trans :
+  Definition bool_copy_TM_trans :
     bool_fin * (Vector.t (option bool_fin) 2) ->
     bool_fin * (Vector.t (option bool_fin * move) 2).
   Proof.
@@ -97,26 +96,26 @@ Section Copy.
       + (* None *) apply (true, [| (None, N); (None, N)|]).
   Defined.
 
-  Definition copy_TM : mTM bool_fin 1.
+  Definition bool_copy_TM : mTM bool_fin 1.
   Proof.
     split with (states := bool_fin).
-    - apply copy_TM_trans.
+    - apply bool_copy_TM_trans.
     - apply false.
     - apply id.
   Defined.
 
-  Definition copy_mTM : { M : mTM bool_fin 1 & states M -> F} := (copy_TM; def).
+  Definition bool_copy_mTM : { M : mTM bool_fin 1 & states M -> F} := (bool_copy_TM; def).
 
-  Lemma copy_TM_onestep (inittapes : tapes bool_fin 2) :
-    cstate (step (M := copy_TM) (initc copy_TM inittapes)) = true.
+  Lemma bool_copy_TM_onestep (inittapes : tapes bool_fin 2) :
+    cstate (step (M := bool_copy_TM) (initc bool_copy_TM inittapes)) = true.
   Proof.
-    unfold initc, step, neg_TM in *. cbn in *.
-    dependent induction inittapes. dependent induction inittapes. cbn in *. clear IHinittapes.
-    destruct (current h); cbn; auto.
+    unfold initc, step, bool_neg_TM in *. destruct_tapes. cbn in *. destruct (current h); cbn; auto.
   Qed.
 
-  Lemma copy_TM_computes_sem :
-    copy_mTM ⊫ computes_locally_R_p (F := F) Fin.F1 Fin.F1 _ _ id.
+  Lemma bool_copy_TM_computes_sem :
+    bool_copy_mTM ⊫
+             (computes_locally_R_p (F := F) Fin.F1 (Fin.FS Fin.F1) _ _ (@id bool)) ∩
+             (stay_locally_R_p (X := bool_fin) (F := F) Fin.F1 _).
   Proof.
     hnf. intros inittapes i (b, outt) HLoop. cbn in *.
     assert (i >= 1).
@@ -126,32 +125,35 @@ Section Copy.
     pose proof loop_fulfills_p HLoop as H_Stop. cbn in *. destruct b; auto.
     unfold loopM in *.
     erewrite (loop_ge (k1 := 1) (k2 := i)) in HLoop. Focus 2. omega. Focus 2.
-    cbn. unfold id. unfold neg_TM. cbn. rewrite copy_TM_onestep. reflexivity. inv HLoop.
-    apply computes_locally_R_iff. hnf. intros x (rest1&E1).
-    unfold initc, step, neg_TM in *. cbn in *.
-    dependent induction inittapes. dependent induction inittapes. cbn in *. clear IHinittapes.
-    hnf.
-    destruct x; cbn in *;
-      erewrite !tape_local_current_cons in H1; eauto; cbn in *; inv H1; cbn in *; now eauto.
+    cbn. unfold id. unfold bool_neg_TM. cbn. rewrite bool_copy_TM_onestep. reflexivity. inv HLoop.
+    unfold initc, step, bool_neg_TM in *. cbn in *.
+    destruct_tapes.
+    unfold computes_locally_R_p, computes_locally_R, tape_encodes_locally, tape_encodes_locally_rest in *.
+    split; cbn.
+    - hnf. intros x (rest1&E1).
+      hnf.
+      destruct x; cbn in *;
+        (erewrite !tape_local_current_cons in H1; eauto); cbn in *; inv H1; cbn in *; now eauto.
+    - hnf. intros x. intros rest1 E1. hnf in *.
+      destruct x; cbn in *;
+        (erewrite !tape_local_current_cons in H1; eauto); cbn in *; inv H1; cbn in *; eauto.
   Qed.
 
-  Lemma copy_TM_computes_terminates_in :
-    copy_TM ↓ (fun _ => fun t => t = 1).
+  Lemma bool_copy_TM_computes_terminates_in :
+    bool_copy_TM ↓ (fun _ => fun t => t = 1).
   Proof.
-    hnf. intros inittape i ->. cbn. unfold id. rewrite copy_TM_onestep. eauto.
+    hnf. intros inittape i ->. cbn. unfold id. rewrite bool_copy_TM_onestep. eauto.
   Qed.
 
-  Lemma copy_TM_computes_total :
-    copy_mTM ⊨(1) computes_locally_R_p (F := F) Fin.F1 Fin.F1 _ _ id.
+  Lemma bool_copy_TM_computes_total :
+    bool_copy_mTM ⊨(1)
+             (computes_locally_R_p (F := F) Fin.F1 (Fin.FS Fin.F1) _ _ (@id bool)) ∩
+             (stay_locally_R_p (X := bool_fin) (F := F) Fin.F1 _).
   Proof.
-    hnf. intros inittape.
-    dependent induction inittape. dependent induction inittape. clear IHinittape; cbn in *.
-    unfold id. rewrite copy_TM_onestep. econstructor. split. eauto.
-    hnf. intros x.
-    rewrite !tape_encodes_locally_iff. unfold tape_encodes_locally'. intros (tape&bl). cbn in *.
-    destruct x; cbn in *; exists tape;
-      cbn; unfold copy_TM, step; cbn;
-        erewrite tape_local_current_cons; eauto; cbn; f_equal; eapply tape_local_right; eauto.
+    hnf. intros inittapes.
+    destruct_tapes; cbn in *.
+    unfold id. rewrite bool_copy_TM_onestep. econstructor. split. eauto.
+    eapply bool_copy_TM_computes_sem. instantiate (1 := 1). cbn. now rewrite bool_copy_TM_onestep.
   Qed.
 
 End Copy.
@@ -162,7 +164,7 @@ Section Dual.
   Variable (F : finType) (def : bool_fin -> F).
   Variable (f : bool * bool -> bool).
 
-  Definition dual_TM_trans :
+  Definition bool_dual_TM_trans :
     bool_fin * (Vector.t (option bool_fin) 2) ->
     bool_fin * (Vector.t (option bool_fin * move) 2).
   Proof.
@@ -173,26 +175,27 @@ Section Dual.
       apply (true, [| (Some (f (b1, b2)), N); (None, N) |]).
   Defined.
 
-  Definition dual_TM : mTM bool_fin 1.
+  Definition bool_dual_TM : mTM bool_fin 1.
   Proof.
     split with (states := bool_fin).
-    - apply dual_TM_trans.
+    - apply bool_dual_TM_trans.
     - apply false.
     - apply id.
   Defined.
 
-  Definition dual_mTM : { M : mTM bool_fin 1 & states M -> F} := (dual_TM; def).
+  Definition bool_dual_mTM : { M : mTM bool_fin 1 & states M -> F} := (bool_dual_TM; def).
 
-  Lemma dual_TM_onestep (inittapes : tapes bool_fin 2) :
-    cstate (step (M := dual_TM) (initc dual_TM inittapes)) = true.
+  Lemma bool_dual_TM_onestep (inittapes : tapes bool_fin 2) :
+    cstate (step (M := bool_dual_TM) (initc bool_dual_TM inittapes)) = true.
   Proof.
-    unfold initc, step, neg_TM in *. cbn in *.
-    dependent induction inittapes. clear IHinittapes. dependent induction inittapes. clear IHinittapes. cbn in *.
+    unfold initc, step, bool_dual_TM in *. destruct_tapes. cbn in *.
     (destruct (current _); cbn; auto); (destruct (current _); cbn; auto).
   Qed.
 
-  Lemma dual_TM_computes_sem :
-    dual_mTM ⊫ computes2_locally_R_p (F := F) Fin.F1 (Fin.FS Fin.F1) Fin.F1 _ _ _ f.
+  Lemma bool_dual_TM_computes_sem :
+    bool_dual_mTM ⊫
+             (stay_locally_R_p (F := F) (Fin.FS Fin.F1) _) ∩
+             computes2_locally_R_p (F := F) Fin.F1 (Fin.FS Fin.F1) Fin.F1 _ _ _ f.
   Proof.
     hnf. intros inittapes i (b, outt) HLoop. cbn in *.
     assert (i >= 1).
@@ -200,51 +203,117 @@ Section Dual.
       destruct i; cbn in *; try discriminate. cbn in *. omega.
     }
     pose proof loop_fulfills_p HLoop as H_Stop. cbn in *. destruct b; auto.
-    unfold loopM in *.
+    unfold id, loopM in *.
     erewrite (loop_ge (k1 := 1) (k2 := i)) in HLoop. Focus 2. omega. Focus 2.
-    cbn. unfold id. unfold dual_TM. cbn. rewrite dual_TM_onestep. reflexivity. inv HLoop.
-    apply computes2_locally_R_iff. hnf. intros x y (rest1&E1) (rest2&E2).
-    unfold initc, step, neg_TM in *. cbn in *.
-    dependent induction inittapes. clear IHinittapes.
-    dependent induction inittapes. clear IHinittapes.
-    dependent induction inittapes. cbn in *.
-    hnf.
-    destruct x, y;
-      (
-        cbn in *;
-        (erewrite tape_local_current_cons in H1; eauto);
-        (erewrite tape_local_current_cons in H1; eauto);
-        cbn in *; inv H1;
-        unfold encode_sum, encode_unit, tape_local; cbn in *;
-        destruct (f (_, _)); now (eexists; cbn; eauto)
-      ).
+    cbn. unfold id. unfold bool_dual_TM. cbn. rewrite bool_dual_TM_onestep. reflexivity. inv HLoop.
+    destruct_tapes; cbn in *.
+    split; cbn; hnf.
+    - intros x. intros rest1 E1. hnf in *.
+      unfold initc, step, bool_neg_TM in *. cbn in *. hnf in *.
+      destruct (current h), x;
+        (
+          unfold encode_sum, encode_unit, tape_local; cbn in *;
+          repeat (erewrite tape_local_current_cons in H1; eauto);
+          cbn in *; inv H1; eauto
+        ).
+    - hnf. intros x y (rest1&E1) (rest2&E2).
+      unfold initc, step, bool_neg_TM in *. cbn in *. hnf in *.
+      destruct x, y;
+        (
+          cbn in *;
+          repeat (erewrite tape_local_current_cons in H1; eauto);
+          cbn in *; inv H1;
+          unfold encode_sum, encode_unit, tape_local; cbn in *;
+          destruct (f (_, _)); now (eexists; cbn; eauto)
+        ).
   Qed.
 
-  Lemma dual_TM_computes_terminates_in :
-    dual_TM ↓ (fun _ => fun t => t = 1).
+  Lemma bool_dual_TM_computes_terminates_in :
+    bool_dual_TM ↓ (fun _ => fun t => t = 1).
   Proof.
-    hnf. intros inittape i ->. cbn. unfold id. rewrite dual_TM_onestep. eauto.
+    hnf. intros inittape i ->. cbn. unfold id. rewrite bool_dual_TM_onestep. eauto.
   Qed.
 
-  Lemma dual_TM_computes_total :
-    dual_mTM ⊨(1) computes2_locally_R_p (F := F) Fin.F1 (Fin.FS Fin.F1) Fin.F1 _ _ _ f.
+  Lemma bool_dual_TM_computes_total :
+    bool_dual_mTM ⊨(1)
+             (stay_locally_R_p (F := F) (Fin.FS Fin.F1) _) ∩
+             computes2_locally_R_p (F := F) Fin.F1 (Fin.FS Fin.F1) Fin.F1 _ _ _ f.
   Proof.
-    hnf. intros inittapes.
-    dependent induction inittapes. clear IHinittapes.
-    dependent induction inittapes. clear IHinittapes.
-    dependent induction inittapes. cbn in *.
-    unfold id. rewrite dual_TM_onestep. econstructor. split. eauto.
-    hnf. intros x y.
-    rewrite !tape_encodes_locally_iff. unfold tape_encodes_locally'. intros (rest1&bl1) (rest2&bl2). cbn in *.
-    destruct x, y;
-      (
-        cbn in *; eexists;
-        unfold dual_TM, step; cbn;
-        (erewrite tape_local_current_cons; eauto);
-        (erewrite tape_local_current_cons; eauto);
-        unfold encode_sum, encode_unit, tape_local; cbn in *;
-        destruct (f (_, _)); (eexists; cbn; eauto)
-      ).
+    hnf. intros inittapes. destruct_tapes. cbn in *.
+    unfold id. rewrite bool_dual_TM_onestep. econstructor. split. eauto.
+    eapply bool_dual_TM_computes_sem. instantiate (1 := 1). cbn. now rewrite bool_dual_TM_onestep.
   Qed.
   
 End Dual.
+
+Require Import TM.Basic.Mono.
+Require Import LiftNM.
+
+Section CopyMove.
+
+  Variable (F : finType) (def : bool_fin -> F).
+
+  Local Definition Move_at_1 := Inject (n := 1) (Move bool_fin R) [| Fin.F1 |] .
+
+  Local Lemma dupfree : Injection.dupfree [| Fin.F1 (n := 1) |].
+  Proof. constructor. inversion 1. constructor. Qed.
+
+  Definition bool_copy_move_mTM := (bool_copy_mTM def ;; Move_at_1).
+
+  Lemma Inj_1_helper : (1 < 2 /\ ~ Vector.In 1 [|0|]).
+  Proof.
+    split.
+    - omega.
+    - inversion 1; subst.
+      apply EqdepFacts.eq_sigT_iff_eq_dep in H3. induction H3. inv H.
+      apply EqdepFacts.eq_sigT_iff_eq_dep in H4. induction H4. destruct_vector. inv H3.
+  Qed.
+
+  Definition bool_copy_move_TM_Sem :
+    bool_copy_move_mTM ⊫ copy_Move_locally_R_p (X := bool_fin) (F := bool_fin) Fin.F1 (Fin.FS Fin.F1) _.
+  Proof.
+    unfold bool_copy_move_mTM, Move_at_1.
+    pose proof (Move_Sem (sig := bool_fin) R).
+    apply WRealise_total in H. cbn in H.
+    pose proof (@Inject_sem bool_fin 0 1 bool_fin (Move bool_fin R) [| Fin.F1 |] dupfree _ H).
+    pose proof (bool_copy_TM_computes_sem (F := F) (def := def)).
+    pose proof (Seq_sem H1 H0).
+    hnf in *. cbn in *. clear H H0 H1. intros t i outc HLoop.
+    specialize (H2 t i outc HLoop). hnf in *.
+    destruct H2 as ((f&midtapes)&(H1&H1')&(H2&H2')). hnf in *. cbn in *.
+    destruct outc.
+    destruct_tapes. cbn in *.
+    unfold id in *. cbn in *.
+    unfold reorder, not_indices in *. unfold Vector.map in *. cbn in *.
+    unfold Match.Match_p in *. cbn in *.
+    split; hnf.
+    - intros x rest HEnc. hnf in *. cbn in *. clear H2'.
+      assert (tape_encodes_locally I_bool h x) as L1 by eauto. specialize (H1 _ L1). clear L1. (* XXX *)
+      destruct cstate as [state | (state & state') ]; cbn in *.
+      + hnf in H2. destruct H2 as (H2&->). hnf in *. subst.
+        enough (rest = nil) as -> by now apply tape_local_nil.
+        unfold tape_encodes_locally_rest in H1'.
+        pose proof (tape_local_nil h1) as (L1&L2).
+        rewrite L2 in H1'; eauto.
+        specialize (H1' x rest HEnc).
+        eapply appendNil; eauto.
+      + destruct (Fin.eqb state' m_true) eqn:E1.
+        * apply Fin.eqb_eq in E1. subst.
+          destruct H2 as (->&(b&H2)).
+          specialize (H1' x rest HEnc). hnf in H1'.
+          eapply tape_local_move_right.
+          destruct x; cbn in *; eauto.
+        * hnf in *. destruct H2 as (H2&H22). hnf in *. subst.
+        enough (rest = nil) as -> by now apply tape_local_nil.
+        pose proof (tape_local_nil h1) as (L1&L2).
+        specialize (H1' x rest HEnc). hnf in H1'.
+        rewrite L2 in H1'; auto.
+        eapply appendNil; eauto.
+    - intros x HEnc. cbn in *. hnf in *. destruct HEnc as (rest&HEnc).
+      assert (tape_encodes_locally I_bool h x) as L1 by eauto. specialize (H1 _ L1). clear L1. (* XXX *)
+      specialize (H1' _ _ HEnc).
+      assert (1 < 2 /\ ~ Vector.In 1 [|0|]) as (L1&L2) by now apply Inj_1_helper.
+      specialize (H2' 1 L1 L2). cbn in *. subst. eauto.
+  Qed.
+  
+End CopyMove.
