TM/Code/Code.v
@@ -1,5 +1,4 @@
 Require Import Prelim.
-Require Import Recdef.
 
 (** * Suffix *)
 
@@ -123,14 +122,7 @@ Proof. destruct 1; [ | apply None]. destruct p. apply Some. constructor. apply x
 Class codeable (X : Type) :=
   {
     encode : encoding_function X;
-    decode : decoding_function X;
     encode_injective : forall (v1 v2 : X) (r1 r2 : list bool), encode v1 ++ r1 = encode v2 ++ r2 -> v1 = v2 /\ r1 = r2;
-    encode_decode : forall (string : list bool) v rest, decode string = Some (v, rest) -> encode v ++ (projT1 rest) = string;
-    decode_encode : forall (v : X) (rest : list bool),
-        match (decode (encode v ++ rest)) with
-        | Some (v', rest') => v = v' /\ projT1 rest' = rest
-        | None => False
-        end;
   }.
 
 
@@ -156,84 +148,6 @@ Proof. destruct v as (a,b). apply (encode_left a ++ encode_right b). Defined.
 Definition encode_unit := fun _ : unit => @nil bool.
 
 
-(** * Basic Decoding Functions *)
-
-Ltac invalid_encoding := apply None.
-
-(** List decoding *)
-
-Lemma decode_list'_helper1 (x : bool) (string : list bool) (ss : list bool)
-      (Rest1 : {rest : list bool & suffix rest ss}) :
-  string = x :: ss -> suffix (projT1 Rest1) string.
-Proof. intros ->. destruct Rest1; cbn. now apply suffix_skip. Qed.
-
-Lemma decode_list'_helper2 (x : bool) (string : list bool) (ss : list bool)
-      (Rest2 : {rest : list bool & suffix rest ss}) :
-      string = x :: ss -> projT1 Rest2 <> string.
-Proof. intros ->. destruct Rest2; cbn. intros ->. eapply suffix_put; eauto. Qed.
-
-Lemma decode_list'_helper3 (x : bool) (string : list bool) (ss : list bool)
-      (Rest1 : {rest : list bool & suffix rest ss})
-      (Rest2 : {rest : list bool & suffix rest (projT1 Rest1)}) :
-  {rest : list bool & suffix rest (x :: ss)}.
-Proof.
-  destruct Rest1 as (rest1, HRest1). destruct Rest2 as (rest2, HRest2). cbn in *.
-  exists rest2. apply suffix_skip. eapply suffix_transitive; eauto.
-Defined.
-
-Function decode_list (X : Type) (decodeEntries : decoding_function X) (string : list bool) {measure length string} :
-  option (list X * {rest : list bool & suffix rest string }) :=
-  match string with
-   | nil =>  None
-   | true  :: ss => 
-     match (decodeEntries ss) with
-     | None => None
-     | Some (dec1, Rest1) =>
-       match
-         @decode_list X decodeEntries (projT1 Rest1) with
-       | None => None
-       | Some (dec2, Rest2) =>
-         Some (dec1 :: dec2, @decode_list'_helper3 true string ss Rest1 Rest2)
-       end
-     end
-   | false :: ss =>  Some (nil, existT _ ss (suffix_skip' _ _))
-   end.
-Proof.
-  intros X decodeEntries string b ss E2 E1 _ dec1 Rest1 _ H.
-  eapply suffix_size_decrease. eapply decode_list'_helper2; eauto. eapply decode_list'_helper1; eauto.
-Defined.
-
-(** Pair decoding *)
-
-Definition decode_pair (X Y : Type) (decode1 : decoding_function X) (decode2 : decoding_function Y) (string : list bool) :
-  option ((X * Y) * {rest : list bool & suffix rest string}).
-Proof.
-  destruct (decode1 string) as [ (dec1, (rest1, HRest1)) | ]; [ | invalid_encoding].
-  destruct (decode2 rest1)  as [ (dec2, (rest2, Hrest2)) | ]; [ | invalid_encoding].
-  do 2 constructor. constructor. apply dec1. apply dec2. exists rest2. eapply suffix_transitive; eauto.
-Defined.
-
-(** Sum decoding *)
-
-Definition decode_sum (X Y : Type) (decode1 : decoding_function X) (decode2 : decoding_function Y) (string : list bool) :
-  option ((X + Y) * {rest : list bool & suffix rest string}).
-Proof.
-  destruct string as [ | s ss].
-  - invalid_encoding.
-  - destruct s eqn:E.
-    + (* Inl = true *)
-      destruct (decode1 ss) as [ (dec, (rest, HRest)) | ]; [ | invalid_encoding].
-      constructor. constructor. left.  apply dec. exists rest. now apply suffix_skip.
-    + (* Inr = false *)
-      destruct (decode2 ss) as [ (dec, (rest, HRest)) | ]; [ | invalid_encoding].
-      constructor. constructor. right. apply dec. exists rest. now apply suffix_skip.
-Defined.
-
-Definition decode_unit (string : list bool) : option (unit * {rest : list bool & suffix rest string}).
-  do 2 constructor. constructor. exists string. apply suffix_full.
-Defined.
-
-
 (** * Basic Coding Instances *) 
 
 (** Lists **)
@@ -248,54 +162,10 @@ Proof.
     * inv H. rewrite <- !app_assoc in H1. apply encode_injective in H1. destruct H1 as (->&H1). apply IH in H1. intuition; congruence.
 Qed.
 
-Lemma encode_decode_list (X : Type) (e : codeable X) (string : list bool) ls rest :
-  decode_list decode string = Some (ls, rest) -> encode_list encode ls ++ (projT1 rest) = string.
-Proof.
-  revert ls rest.
-  pose proof (suffix_induction_provider string) as ind.
-  induction ind as [ xs H IH]; rewrite !decode_list_equation; intros ls rest H1; rewrite <- decode_list_equation in *.
-  destruct xs as [ | x ss] eqn:E; try discriminate.
-  destruct x; rewrite !decode_list_equation in *.
-  - destruct (decode ss) as [(dec1, Rest1)| ] eqn:E2; try discriminate; simpl in *.
-    destruct (decode_list decode (projT1 Rest1))
-      as [(dec2, Rest2)| ] eqn:E3; try discriminate. inv H1.
-    apply IH in E3; auto.
-    + destruct Rest1, Rest2. simpl in *. f_equal.
-      rewrite <- app_assoc. rewrite E3.
-      erewrite <- encode_decode; eauto.
-      cbn. reflexivity.
-    + eapply decode_list'_helper1; eauto.
-    + eapply decode_list'_helper2; eauto.
-  - inv H1. cbn. reflexivity.
-Qed.
-
-Lemma decode_encode_list (X : Type) (e : codeable X) :
-  forall (v : list X) (rest : list bool),
-    match (decode_list decode (encode_list encode v ++ rest)) with
-    | Some (v', rest') => v = v' /\ projT1 rest' = rest
-    | None => False
-    end.
-Proof.
-  intros v rest.
-  revert rest.
-  induction v as [ | v vs IH]; intros rest; rewrite !decode_list_equation; simpl.
-  - auto.
-  - rewrite <- !app_assoc in *.
-    pose proof (decode_encode v (encode_list encode vs ++ rest)) as E1'.
-    destruct (decode (encode v ++ encode_list encode vs ++ rest)) as [(dec1&rest1&Hrest1)| ] eqn:E1; auto.
-    simpl in *. destruct E1' as (->&->).
-    specialize (IH rest).
-    destruct (decode_list decode (encode_list encode vs ++ rest)) as [(dec2&rest2&Hrest2)| ]; auto.
-    simpl in *. destruct IH as (->&->). auto.
-Qed.
-
-
 Instance I_list (X : Type) (e1 : codeable X) : codeable (list X).
 Proof.
-  split with (encode := encode_list encode) (decode := decode_list decode).
+  split with (encode := encode_list encode).
   - apply encode_injective_list.
-  - apply encode_decode_list.
-  - apply decode_encode_list.
 Defined.
 
 
@@ -308,44 +178,10 @@ Proof.
   apply encode_injective in H as (->&H). apply encode_injective in H as (->&->). auto.
 Qed.
 
-Lemma encode_decode_pair (X Y : Type) (e1 : codeable X) (e2 : codeable Y) (string : list bool) (v : X * Y) rest :
-  decode_pair decode decode string = Some (v, rest) -> encode_pair encode encode v ++ (projT1 rest) = string.
-Proof.
-  intros H. destruct v as (a, b).
-  unfold encode_pair, decode_pair in *.
-  destruct (decode string) as [(cod1, (rest1, HRest1))| ] eqn:E1; cbn in *; try discriminate.
-  destruct (decode rest1) as [(cod2, (rest2, HRest2))| ] eqn:E2; cbn in *; try discriminate.
-  inv H. cbn in *.
-  pose proof (@encode_decode X e1) as IH1. pose proof (@encode_decode Y e2) as IH2.
-  specialize (IH1 _ _ _ E1). cbn in *. specialize (IH2 _ _ _ E2). cbn in *.
-  subst. symmetry. now apply app_assoc.
-Qed.
-
-Lemma decode_encode_pair (X Y : Type) (e1 : codeable X) (e2 : codeable Y) :
-  forall (v : X * Y) (rest : list bool),
-    match (decode_pair decode decode (encode_pair encode encode v ++ rest)) with
-    | Some (v', rest') => v = v' /\ projT1 rest' = rest
-    | None => False
-    end.
-Proof.
-  intros (a, b) rest. unfold decode_pair, encode_pair.
-  rewrite <- app_assoc in *.
-  pose proof (decode_encode a (encode b ++ rest)) as E'.
-  destruct (decode (encode a ++ encode b ++ rest)) as [(dec1&rest1&Hrest1)| ] eqn:E; cbn in *.
-  - destruct E' as (->&->).
-    pose proof (decode_encode b rest) as E2'.
-    destruct (decode (encode b ++ rest) ) as [(dec2&rest2&Hrest2)| ] eqn:E2; cbn in *.
-    + destruct E2' as (->&->). auto.
-    + auto.
-  - auto.
-Qed.
-
 Instance I_pair (X Y : Type) (e1 : codeable X) (e2 : codeable Y) : codeable (X * Y).
 Proof.
-  split with (encode := encode_pair encode encode) (decode := decode_pair decode decode).
+  split with (encode := encode_pair encode encode).
   - apply encode_injective_pair.
-  - apply encode_decode_pair.
-  - apply decode_encode_pair.
 Defined.
 
 
@@ -357,49 +193,10 @@ Proof.
   intros [v1|v1] [v2|v2] r1 r2; unfold encode_sum; intros H1; cbn in *; inv H1; apply encode_injective in H0; intuition; congruence.
 Qed.
 
-Lemma encode_decode_sum (X Y : Type) (e1 : codeable X) (e2 : codeable Y) (string : list bool) (v : X + Y) rest :
-  decode_sum decode decode string = Some (v, rest) -> encode_sum encode encode v ++ (projT1 rest) = string.
-Proof.
-  intros H. destruct v as [v1|v2].
-  + destruct string; try discriminate; cbn in *.
-    destruct b; try discriminate.
-    * destruct (decode string) eqn:E; cbn in *; try discriminate.
-      destruct p, s. inv H.
-      apply encode_decode in E. cbn in *. congruence.
-    * destruct (decode string) eqn:E; cbn in *; try discriminate.
-      destruct p, s. inv H.
-  + destruct string; try discriminate; cbn in *.
-    destruct b; try discriminate.
-    * destruct (decode string) eqn:E; cbn in *; try discriminate.
-      destruct p, s. inv H.
-    * destruct (decode string) eqn:E; cbn in *; try discriminate.
-      destruct p, s. inv H. apply encode_decode in E. cbn in *. congruence.
-Qed.
-
-Lemma decode_encode_sum (X Y : Type) (e1 : codeable X) (e2 : codeable Y) :
-  forall (v : X + Y) (rest : list bool),
-    match (decode_sum decode decode (encode_sum encode encode v ++ rest)) with
-    | Some (v', rest') => v = v' /\ projT1 rest' = rest
-    | None => False
-    end.
-Proof.
-  intros [a|a] rest.
-  - unfold decode_sum, encode_sum. cbn in *.
-    pose proof (decode_encode a rest) as E'.
-    destruct (decode (encode a ++ rest)) as [(dec1&rest1&Hreset1) | ]; auto.
-    intuition; congruence.
-  - unfold decode_sum, encode_sum. cbn in *.
-    pose proof (decode_encode a rest) as E'.
-    destruct (decode (encode a ++ rest)) as [(dec1&rest1&Hreset1) | ]; auto.
-    intuition; congruence.
-Qed.
-
 Instance I_sum (X Y : Type) (e1 : codeable X) (e2 : codeable Y) : codeable (X + Y).
 Proof.
-  split with (encode := encode_sum encode encode) (decode := decode_sum decode decode).
+  split with (encode := encode_sum encode encode).
   - apply encode_injective_sum.
-  - apply encode_decode_sum.
-  - apply decode_encode_sum.
 Defined.
 
 
@@ -409,28 +206,10 @@ Lemma encode_injective_unit :
   forall (v1 v2 : unit) (r1 r2 : list bool), encode_unit v1 ++ r1 = encode_unit v2 ++ r2 -> v1 = v2 /\ r1 = r2.
 Proof. intros () () r1 r2. auto. Qed.
 
-Lemma encode_decode_unit (string : list bool) (v : unit) rest :
-  decode_unit string = Some (v, rest) -> encode_unit v ++ (projT1 rest) = string.
-Proof.
-  destruct v, rest. unfold decode_unit, encode_unit in *. intros H. inv H; cbn. reflexivity.
-Qed.
-
-Lemma decode_encode_unit :
-  forall (v : unit) (rest : list bool),
-    match (decode_unit (encode_unit v ++ rest)) with
-    | Some (v', rest') => v = v' /\ projT1 rest' = rest
-    | None => False
-    end.
-Proof.
-  destruct v, rest; unfold decode_unit, encode_unit in *; auto.
-Qed.
-
 Instance I_unit : codeable unit.
 Proof.
-  split with (encode := encode_unit) (decode := decode_unit).
+  split with (encode := encode_unit).
   - apply encode_injective_unit.
-  - apply encode_decode_unit.
-  - apply decode_encode_unit.
 Defined.
 
 
@@ -438,75 +217,25 @@ Defined.
 
 Class Cast (X Y : Type) :=
   {
-    cast1 : X -> Y;
-    cast2 : Y -> X;
-    cast_adj1 : forall (x : X), cast2 (cast1 x) = x;
-    cast_adj2 : forall (y : Y), cast1 (cast2 y) = y;
+    cast : Y -> X;
+    cast_injective : forall x1 x2, cast x1 = cast x2 -> x1 = x2;
   }.
 
-Lemma adj_inj (X Y : Type) (f : X -> Y) (g : Y -> X) :
-  (forall (x : X), g (f x) = x) -> injective f.
-Proof.
-  intros H x1 x2 H2. rewrite <- (H x1), <- (H x2). rewrite H2. reflexivity.
-Qed.
-
 Section I_Cast.
-  Variable (X Y : Type) (cast : Cast X Y) (e : codeable X).
-  Definition encode_cast := fun y => encode (cast2 y).
-  Definition decode_cast := fun string => let try out' := decode string in let (dec, rest) := out' in Some (cast1 dec, rest).
+  Variable (X Y : Type) (castXY : Cast X Y) (e : codeable X).
 
-  Lemma encode_injective_cast :
-    forall (v1 v2 : Y) (r1 r2 : list bool),
-      encode_cast v1 ++ r1 = encode_cast v2 ++ r2 -> v1 = v2 /\ r1 = r2.
-  Proof.
-    intros v1 v2 r1 r2 H. eapply encode_injective in H as (H&->). split; auto. eapply adj_inj; eauto. eapply cast_adj2.
-  Qed.
-  
-  Lemma encode_decode_cast:
-    forall (string : list bool) (v : Y)
-      (rest : {rest : list bool & suffix rest string}),
-      decode_cast string = Some (v, rest) ->
-      encode_cast v ++ projT1 rest = string.
-  Proof.
-    unfold decode_cast, encode_cast. cbn in *.
-    intros string v rest H. apply encode_decode.
-    eapply adj_inj.
-    instantiate (1 := fun out => let try out' := out in let (dec, rest) := out' in Some (cast1 dec, rest)).
-    instantiate (1 := fun out => let try out' := out in let (dec, rest) := out' in Some (cast2 dec, rest)).
-    - intros xs. cbn. destruct xs; auto. destruct p. now rewrite cast_adj1.
-    - cbn. now rewrite cast_adj2.
-  Qed.
-
-  Lemma decode_encode_cast:
-    forall (v : Y) (rest : list bool),
-      match decode_cast (encode_cast v ++ rest) with
-      | Some (v', rest') => v = v' /\ projT1 rest' = rest
-      | None => False
-      end.
-  Proof.
-    unfold decode_cast, encode_cast. cbn in *.
-    intros v rest.
-    destruct (decode (encode (cast2 v) ++ rest)) as [(dec, Rest)| ] eqn:E1.
-    - pose proof (decode_encode (cast2 v) rest). rewrite E1 in H. destruct H. split; auto.
-      eapply adj_inj with (f := cast2) (g := cast1). apply cast_adj2. rewrite <- H. now rewrite cast_adj2.
-    - pose proof (decode_encode (cast2 v) rest). now rewrite E1 in H.
-  Qed.
-  
   Lemma I_cast : codeable Y.
   Proof.
-    esplit with (encode := encode_cast) (decode := decode_cast).
-    - apply encode_injective_cast.
-    - apply encode_decode_cast.
-    - apply decode_encode_cast.
+    esplit with (encode := fun y => encode (cast y)).
+    - intros v1 v2 r1 r2 H. apply encode_injective in H as (H&->). split; auto. now apply cast_injective in H.
   Defined.
 
 End I_Cast.
 
 Instance cast_bool : Cast (unit + unit) bool.
 Proof.
-  split with (cast1 := fun p => match p with inl _ => true | inr _ => false end) (cast2 := fun (b : bool) => if b then inl tt else inr tt).
-  - intros [()|()]; auto.
-  - intros b. destruct b; auto.
+  split with (cast := fun (b : bool) => if b then inl tt else inr tt).
+  - intros x1 x2 H. destruct x1, x2; auto; congruence.
 Defined.
 
 Instance I_bool : codeable bool.
@@ -514,41 +243,65 @@ Proof. eapply I_cast. eapply cast_bool. auto. Defined.
 
 Instance cast_option (X : Type) : Cast (X + unit) (option X).
 Proof.
-  split with (cast1 := fun p => match p with inl x => Some x | inr _ => None end)
-             (cast2 := fun p => match p with Some x => inl x | None => inr tt end).
-  - intros [x|()]; auto.
-  - intros [x|  ]; auto.
+  split with (cast := fun p => match p with Some x => inl x | None => inr tt end).
+  - intros [x|  ] [y| ] H; auto; congruence.
 Defined.
 
 Instance I_option (X : Type) : codeable X -> codeable (option X).
 Proof. intros H. eapply I_cast. eapply cast_option. auto. Defined.
 
-Lemma repeat_length_unit:
-  forall xs : list unit, repeat tt (| xs |) = xs.
-Proof. intros xs. induction xs; cbn; auto. destruct a. f_equal. assumption. Qed.
+Lemma repeat_surjective (X : Type) (x : X) (n m : nat) :
+  repeat x n = repeat x m -> n = m.
+Proof.
+  revert m. induction n; intros m H.
+  - destruct m; cbn in *; congruence.
+  - cbn in *. destruct m; cbn in *. congruence. f_equal. apply IHn. congruence.
+Qed.
 
 Instance cast_nat : Cast (list unit) nat.
 Proof.
-  split with (cast1 := @List.length unit) (cast2 := @List.repeat unit tt).
-  - apply repeat_length_unit.
-  - intros y. apply List.repeat_length.
+  split with (cast := @List.repeat unit tt).
+  - apply repeat_surjective.
 Defined.
 
 Instance I_nat : codeable nat.
 Proof. eapply I_cast. eapply cast_nat. auto. Defined.
 
+Section Fin.
+
+  Variable (n : nat).
+
+  Definition fin_to_nat : (Fin.t n) -> nat :=
+    fun i :  (Fin.t n) => proj1_sig (Fin.to_nat i).
+  
+  Lemma fin_to_nat_injective:
+    forall x1 x2 : (Fin.t n),
+      fin_to_nat x1 = fin_to_nat x2 -> x1 = x2.
+  Proof.
+    intros x1 x2. unfold fin_to_nat. intros H.
+    f_equal. now apply Fin.to_nat_inj.
+  Qed.
+  
+  Instance cast_Fin : Cast nat (Fin.t n).
+  Proof.
+    split with (cast := fin_to_nat).
+    apply fin_to_nat_injective.
+  Defined.
+
+  Instance I_Fin : codeable (Fin.t n).
+  Proof. eapply I_cast. eapply cast_Fin. auto. Defined.
+  
+End Fin.
+
 (** Test Playground *)
 
 (*
-Compute decoding_output_project (decode (X := unit) (encode tt)).
-Compute decoding_output_project (decode (X := unit) (encode (tt, tt))).
-
 Compute (encode (X := list unit * (unit + unit) * (unit + unit)) ([tt;tt;tt], inr tt, inl tt)).
-Compute decoding_output_project (decode (X := list unit * (unit + unit) * (unit + unit)) (encode ([tt;tt;tt], inr tt, inl tt))).
 
 Compute encode [true; false].
 Compute encode [inl (Some (true)); inl None; inr tt].
 
 Compute (encode (Some [inl (Some (true)); inl None; inr 42])).
-Compute decoding_output_project (decode (X := option (list (option (bool) + nat))) (encode (Some [inl (Some (true)); inl None; inr 42]))).
+
+Compute (@encode _ (I_Fin 10) (Fin.FS (Fin.FS (Fin.FS (Fin.F1))))).
 *)
